src/OneLoop.py
@@ -1,11 +1,11 @@
 from z3 import *
 
 L = [
-lambda x :(True and (x[2] > 0)),
-lambda x :[((3 * x[0]) - (4 * x[1])), ((4 * x[0]) + (3 * x[1])), ((x[2] + x[0]) - 1), x[0], ],
-4,
+lambda x :(((True and (True and (x[0] < 10)) ) if (x[0] < 10) else (True and (True and (not(x[0] < 10))) ) ) and (True and (x[0] != 0)) ),
+lambda x :[((x[0] + 1) if (x[0] < 10) else (x[1] - 1) ), ((x[1] - 1) if (x[0] < 10) else (x[1] - 1) ), ],
+2,
 0,
-lambda x :[( ( 3* x[0])- ( 4* x[1])), ( ( 4* x[0])+ ( 3* x[1])), ( ( x[2]+ x[0])- 1), x[0], ],
-lambda x :(And( True, ( x[2]> 0))),
+lambda x :[If(( x[0]< 10), ( x[0]+ 1), ( x[1]- 1) ), If(( x[0]< 10), ( x[1]- 1), ( x[1]- 1) ), ],
+lambda x :And(If(( x[0]< 10), And(True, (And( True, ( x[0]< 10))) ), And(True, (And( True, (Not(x[0] < 10)))) ) ), (And( True, ( x[0]!= 0))) ),
 False,
 ]
