src/svmranker_last_input.bpl
@@ -1,0 +1,17 @@
+function __VERIFIER_nondet_int() returns (int);
+procedure main()
+{
+  var x: int;
+  var y: int;
+  x := __VERIFIER_nondet_int();
+  y := __VERIFIER_nondet_int();
+  while (((x > 0) && (y > 0)))
+  {
+  if ((__VERIFIER_nondet_int() != 0))
+  {
+    x := (x - 1);
+    y := (2 * y);  } else {
+    y := (y - 1);  }
+  }
+
+}
