temp.bpl
@@ -1,11 +1,12 @@
+function __VERIFIER_nondet_int() returns (int);
 procedure main()
 {
   var x: int;
   var y: int;
   x := __VERIFIER_nondet_int();
   y := __VERIFIER_nondet_int();
-  while ((((x>0)&&(x>y))&&(y<=(2147483647-x))))
+  while ((((x > 0) && (x > y)) && (y <= (2147483647 - x))))
   {
-  y := (y+x);  }
+  y := (y + x);  }
 
 }
